src/Examples/Executable/Interval/Example_Interval_DG_IP_Flagship.thy
@@ -7,12 +7,8 @@ theory Example_Interval_DG_IP_Flagship
     "Voblint_CFG.IMP2_Proc_to_CFG"
     "Voblint_Analysis.Analysis_GraphViz"
     "Voblint_IMP2.IMP2_Notation"
-    "Voblint_IMP2.IMP2_Bridge"
     "Voblint_Formalization.Source_Activation_Sound"
 begin
-
-no_notation Syntax.Assign (\<open>_ ::= _\<close> [1000, 61] 61)
-hide_const (open) Syntax.N Syntax.V
 
 definition twice_program :: imp_prog where
   "twice_program = program {
